1.If (2)^1/2 is rational, then we can write (2)^1/2 = a/b, where b does not equal 0.
  -The equation can be rewritten as 2 = a^2/b^2
  -a/b are in there most simplified forms
  -a can only be even if b is odd, or it can be odd only if b is even.
  -If a is even then a = 2k.
  -If a = 2k, 2 = ([2k]^2)/b^2 =
   2b^2 = 4k^2
   b^2 = 2k^2
   b = 2k
  -Given the conclusion above, we can see that b is in fact even. But b cannot be even
   when a is even if a/b are already in their simplest forms.
  -Therefore (2)^1/2 is not rational,  proven by contradiction
2. Given:  If n = 25, 100, or 169, then n is a perfect square and is the sum of two perfect squares.
  - Let n = 25, 100, 169
  - m = 5, 10, 132
  - m^2 = 25, 100, 169
  -n is a perfect square if it is 25, 100, or 169 
  
  - 4^2 + 3^2 = 25, 8^2 + 6^2 = 100, 12^2 + 5^2 = 169
  - 16 + 9 = 25, 64 + 36 = 100, 144 + 25 = 169
  -n is the sum of 2 perfect squares.
  -These two have both been proven by exhuastion.

3. Given: The sum of two odd integers is even. Hint: By definition, even integers can be expressed as 2n, thus odd integers can be expressed as 2n + 1
 - If the sum of 2 odd integers is not even, then the sum of 2 odd
   integers is odd, or (2n+1) + 2n+1 = (2n+1) where n is any integer.
 - if n = 3, then 6+1 + 6+1 = 6+1 or 7+7 = 7 or 14 = 7
 - Because 14=/=7, the sum of two odd integers cannot be another odd number, therefore
   the sum of two odd integers is even. Proven by contradiction.
	                
4. The sum of an even integer and it's square is even
     x = 2n, y = 4n^2
     x+y = 2m
   - 2n + (2n)^2
   - 2n + 4n^2 
   - 2(n+2n^2)
   - let (n+n^2) = k
   - x+y = 2k
    x+y is even by definition of an even integer. Proven by direct proof.
	
5. Given: If x squared is odd, then x is odd
   - let x = 2n+1
   - (2n+1)(2n+1) = (4n)^2 + 4n + 1
   - 2(2n^2+2n) + 1
   - let 2n^2+2n = k
   - 2k+1
   x^2 is odd if x is odd, proven by direct proof.    


1. Prove by induction that 1 + 5 + 9 + ... + (4n-3) = n(2n-1)
   1 = 1[2(1)-1]
   1 = 1(1)
   base case is true
   k(2k-1) + 4(k+1) - 3 = (k+1)(2[k+1]-1)  
   k(2k-1) + 4(k+1) - 3 = (k+1)(2k+2-1)                     
   k(2k-1) + 4(k+1) - 3 = (k+1)(2k+1)
   2k^2-k+4k+1 = 2k^2+k+2k+1
   2k^2+3k+1 = 2k^2+3k+1
   We have proven that, if k is true,  then k+1 is true.

2. Prove that for any positive integer number n, n^3 + 2n is divisible by 3
   (1)^3 + 2(1) = 1+2
              = 3
              = 3*1
   k^3 + 2k = 3m
   (k+1)^3 + 2(k+1) = 3m
   (k^2+2k+1)(k+1) + 2(k+1) = 3m
   (k^3 + 2k^2 + k + k^2 + 2k + 1) + 2(k+1) = 3m
   k^3 + 3k^2 + 3k + 1 + 2k+2 = 3m
   k^3 + 2k+ 3k^3 + 3k + 3 = 3m
   3m + 3k^3 + 3k + 3 = 3m
   3(m + k^3 + k + 1) = 3m
   let m + k^3 + k + 1 = n
   3n = 3m
   n = m
   Proven through induction.


3.Prove that for n >= 1, 9^n - 1 is divisible by 8 for all non-negative integers Hint: 4^(3+1) = 4 * 4^3 Hint: If 9^n - 1 = 8m, then 9^n = 8m + 1








   
